src/lib/kuiper/Kuiper.Array.fsti
@@ -362,6 +362,21 @@ fn gpu_slice_gather
     forall+ (_:natlt k). gpu_pts_to_slice arr #(f /. Real.of_int k) m n 'v
   ensures gpu_pts_to_slice arr #f m n 'v
 
+ghost
+fn gpu_slice_pts_to_eq
+  (#a:Type u#0)
+  (#sz:nat)
+  (arr : gpu_array a sz)
+  (m n:nat)
+  (#f1 f2 : perm)
+  (#v1 #v2 : seq a)
+  requires
+    gpu_pts_to_slice arr #f1 m n v1 **
+    gpu_pts_to_slice arr #f2 m n v2
+  ensures
+    gpu_pts_to_slice arr #f1 m n v2 **
+    gpu_pts_to_slice arr #f2 m n v2
+
 val adjacent
   (#a : Type u#0)
   (#s1 #s2 : nat)
